

3.a)Question:Prove that $R(\theta)^T R(\theta) = I \forall \theta$ Solution:

$$\begin{aligned}
R(\theta)^T R(\theta) &= \begin{pmatrix} \cos(\theta) & \sin(\theta) \\ -\sin(\theta) & \cos(\theta) \end{pmatrix} \begin{pmatrix} \cos(\theta) & -\sin(\theta) \\ \sin(\theta) & \cos(\theta) \end{pmatrix} = \begin{pmatrix} \cos^2(\theta) + \sin^2(\theta) & -\sin(\theta)\cos(\theta) + \sin(\theta)\cos(\theta) \\ -\sin(\theta)\cos(\theta) + \sin(\theta)\cos(\theta) & \cos^2(\theta) + \sin^2(\theta) \end{pmatrix} \\
&= \begin{pmatrix} 1 & 0 \\ 0 & 1 \end{pmatrix} = I \\
\therefore R(\theta)^T R(\theta) &= I \forall \theta
\end{aligned}$$

3.b)Question:Prove that $\det(R(\theta)) = 1 \forall \theta$ Solution:

$$\begin{aligned}
\det(R(\theta)) &= \det \begin{pmatrix} \cos(\theta) & -\sin(\theta) \\ \sin(\theta) & \cos(\theta) \end{pmatrix} = \cos^2(\theta) + \sin^2(\theta) = 1 \\
\therefore \det(R(\theta)) &= 1 \forall \theta
\end{aligned}$$

3.c)Question:Derive the inverse $R(\theta)^{-1}$ and show it equals $R(-\theta)$ Solution:

The inverse of $R(\theta)$ is the rotation matrix that when multiplied with $R(\theta)$ results in the identity matrix. This inverse is the transpose of $R(\theta)$ as seen by part 3.a.

$$\begin{aligned}
R(\theta)^{-1} &= R(\theta)^T = \begin{pmatrix} \cos(\theta) & \sin(\theta) \\ -\sin(\theta) & \cos(\theta) \end{pmatrix} \\
R(-\theta) &= \begin{pmatrix} \cos(-\theta) & -\sin(-\theta) \\ \sin(-\theta) & \cos(-\theta) \end{pmatrix} = \begin{pmatrix} \cos(\theta) & \sin(\theta) \\ -\sin(\theta) & \cos(\theta) \end{pmatrix} = R(\theta)^{-1} \\
\therefore R(\theta)^{-1} &= R(-\theta)
\end{aligned}$$

3.d)Question:Prove that $R(\theta_1)R(\theta_2) = R(\theta_1 + \theta_2)$ Solution:

$$\begin{aligned}
R(\theta_1)R(\theta_2) &= \begin{pmatrix} \cos(\theta_1) & -\sin(\theta_1) \\ \sin(\theta_1) & \cos(\theta_1) \end{pmatrix} \begin{pmatrix} \cos(\theta_2) & -\sin(\theta_2) \\ \sin(\theta_2) & \cos(\theta_2) \end{pmatrix} \\
&= \begin{pmatrix} \cos(\theta_1)\cos(\theta_2) - \sin(\theta_1)\sin(\theta_2) & -\cos(\theta_1)\sin(\theta_2) - \sin(\theta_1)\cos(\theta_2) \\ \sin(\theta_1)\cos(\theta_2) + \cos(\theta_1)\sin(\theta_2) & -\sin(\theta_1)\sin(\theta_2) + \cos(\theta_1)\cos(\theta_2) \end{pmatrix} \\
&= \begin{pmatrix} \cos(\theta_1 + \theta_2) & -\sin(\theta_1 + \theta_2) \\ \sin(\theta_1 + \theta_2) & \cos(\theta_1 + \theta_2) \end{pmatrix} = R(\theta_1 + \theta_2) \\
\therefore R(\theta_1)R(\theta_2) &= R(\theta_1 + \theta_2)
\end{aligned}$$

3.e)

Question:

Is $\text{SO}(2)$ an abelian group?

Solution:

An abelian group is defined by a group where the group operation commutes. If $\text{SO}(2)$ commutes then $R(\theta_1)R(\theta_2) = R(\theta_2)R(\theta_1)$

$$\text{from 3.d we know } R(\theta_1)R(\theta_2) = R(\theta_1 + \theta_2) = R(\theta_2 + \theta_1) = R(\theta_2)R(\theta_1)$$

Therefore, $\text{SO}(2)$ commutes so it is an abelian group.